Iris/IrisTest/Embedding.lean
@@ -72,69 +72,63 @@ example [BIUpdate PROP1]
   Tests `FromModal` instances with the selector not fixed.
   The default instance `modality_embed` is used.
 -/
-/-- info: solution:
-  FromModal FromModal.ModalityStatus.matchGoal True modality_embed
-    ⎡<affine> P⎤ ⎡<affine> P⎤ iprop(<affine> P), new goals: []
+/--
+info: solution: FromModal InOut.out modality_embed True ⎡<affine> P⎤ ⎡<affine> P⎤ iprop(<affine> P), new goals: []
 -/
 #guard_msgs (whitespace := lax) in
 variable (P : PROP1) in
-#ipm_synth FromModal .matchGoal (α := PROP2) _ _ _ iprop(⎡<affine> P⎤ : PROP2) _
+#ipm_synth FromModal .out (α := PROP2) _ _ _ iprop(⎡<affine> P⎤ : PROP2) _
 
 /-
   Tests `FromModal` instances with the selector fixed: the low priority
   instances are reachable only once the selector rules out `modality_embed`.
 -/
-/-- info: solution:
-FromModal FromModal.ModalityStatus.matchGoal True
-  modality_intuitionistically iprop(□ P) ⎡□ P⎤ ⎡P⎤, new goals: []
+/--
+info: solution: FromModal InOut.out modality_intuitionistically True iprop(□ P) ⎡□ P⎤ ⎡P⎤, new goals: []
 -/
 #guard_msgs (whitespace := lax) in
 variable (P : PROP1) in
-#ipm_synth FromModal .matchGoal _ _ iprop(□ P) iprop(⎡□ P⎤ : PROP2) _
+#ipm_synth FromModal .out _ _ iprop(□ P) iprop(⎡□ P⎤ : PROP2) _
 
 /-
   Tests `FromModal` synthesis that is done by `fromModal_intuitionistically_embed`,
   with `io = InOut.in`.
 -/
-/-- info: solution:
-FromModal FromModal.ModalityStatus.known True
-  modality_intuitionistically iprop(□ P) iprop(□ P) P, new goals: []
+/--
+info: solution: FromModal InOut.in modality_intuitionistically True iprop(□ P) iprop(□ P) P, new goals: []
 -/
 #guard_msgs (whitespace := lax) in
 variable (P : PROP1) in
-#ipm_synth FromModal .known _ modality_intuitionistically iprop(□ P) iprop(□ P : PROP1) _
+#ipm_synth FromModal .in modality_intuitionistically _ iprop(□ P) iprop(□ P : PROP1) _
 
 /- Tests `FromModal` synthesis with `io = InOut.in` along with an unfixed selector. -/
-/-- info: solution:
-FromModal FromModal.ModalityStatus.known True modality_id
-  iprop(|==> P) iprop(|==> P) P, new goals: []
+/--
+info: solution: FromModal InOut.in modality_id True iprop(|==> P) iprop(|==> P) P, new goals: []
 -/
 #guard_msgs (whitespace := lax) in
 variable (P : PROP1) [BIUpdate PROP1] in
-#ipm_synth FromModal .known (α := PROP1) _ modality_id _ iprop(|==> P : PROP1) _
+#ipm_synth FromModal .in (α := PROP1) modality_id _ _ iprop(|==> P : PROP1) _
 
 /-
   Tests `FromModal` synthesis with nested embeddings.
 -/
-/-- info: solution:
-FromModal FromModal.ModalityStatus.matchGoal True modality_affinely
-  iprop(<affine> P) ⎡⎡<affine> P⎤⎤ ⎡⎡P⎤⎤, new goals: []
+/--
+info: solution: FromModal InOut.out modality_affinely True iprop(<affine> P) ⎡⎡<affine> P⎤⎤ ⎡⎡P⎤⎤, new goals: []
 -/
 #guard_msgs (whitespace := lax) in
 variable {PROP3 : Type u} [BI PROP3] [BiEmbed PROP2 PROP3] (P : PROP1) in
-#ipm_synth FromModal .matchGoal _ _ iprop(<affine> P) iprop(⎡(⎡<affine> P⎤ : PROP2)⎤ : PROP3) _
+#ipm_synth FromModal .out _ _ iprop(<affine> P) iprop(⎡(⎡<affine> P⎤ : PROP2)⎤ : PROP3) _
 
 /-
   Tests `FromModal` synthesis with the `InOut` parameter not matching the fact
   that `PROP1` is supplied.
 -/
-/-- error:
-parameter #1 PROP1 of FromModal FromModal.ModalityStatus.matchGoal ?m.7 ?m.8 iprop(□ P) iprop(□ P)
-  ?m.13 is an out parameter that is not an mvar
+/--
+error: parameter #1 PROP1 of FromModal InOut.out ?m.7 ?m.8 iprop(□ P) iprop(□ P) ?m.13 is an out parameter that is not an mvar
 -/
 #guard_msgs (whitespace := lax) in
 variable (P : PROP1) in
-#ipm_synth FromModal (PROP1 := PROP1) .matchGoal _ _ iprop(□ P) iprop(□ P : PROP1) _
+#ipm_synth FromModal (PROP1 := PROP1) .out _ _ iprop(□ P) iprop(□ P : PROP1) _
 
 /-
   Same test as about, except `io = InOut.in`.
@@ -143,7 +137,7 @@ variable (P : PROP1) in
 /-- info: None -/
 #guard_msgs in
 variable (P : PROP1) in
-#ipm_synth FromModal .known (α := PROP1) _ _ iprop(□ P) iprop(□ P : PROP1) _
+#ipm_synth FromModal .in (α := PROP1) _ _ iprop(□ P) iprop(□ P : PROP1) _
 
 /-
   Tests `imodintro` with the selection for `FromModal` fixed.
@@ -264,7 +258,6 @@ variable (P : PROP1) (φ : Prop) in
 -/
 #guard_msgs (whitespace := lax) in
 variable [BiEmbedEmp PROP1 PROP2] (P : PROP1) in
--- set_option trace.Meta.synthInstance true in
 #ipm_synth Frame (PROP := PROP2) true iprop(⎡P⎤) iprop(⎡□ P⎤) _
 
 /- The instance `frame_here_pure_persistent` has a higher priority than `frame_pure_embed`. -/
